Add an initial disk model
Just the syntax, no semantics yet

src/Goose/GoLayer.v
@@ -8,17 +8,21 @@ From Perennial Require Import Helpers.RecordZoom.
 From Perennial Require Import Spec.Proc.
 From Perennial Require Import Spec.InjectOp.
 From Perennial Require Import Spec.Layer.
-From Perennial.Goose Require Export Machine Heap Filesys Globals.
+From Perennial.Goose Require Export Machine Heap Filesys Globals Disk.
 
 Inductive Op `{GoModel} : Type -> Type :=
 | FilesysOp : forall T, FS.Op T -> Op T
 | DataOp : forall T, Data.Op T -> Op T
 | LockGlobalOp : forall T, Globals.Op (slice.t LockRef) T -> Op T
+(* TODO: we will need to separate out Goose with a filesys and Goose with a
+   disk, since they each depend on the heap *)
+| DiskOp : forall T, Disk.Op T -> Op T
 .
 
 Instance data_inj `{GoModel} : Injectable Data.Op Op := DataOp.
 Instance fs_inj `{GoModel} : Injectable FS.Op Op := FilesysOp.
 Instance lock_global_inj `{GoModel} : Injectable (Globals.Op (slice.t LockRef)) Op := LockGlobalOp.
+Instance disk_global_inj `{GoModel} : Injectable Disk.Op Op := DiskOp.
 
 Module Go.
   Section GoModel.
@@ -27,13 +31,14 @@ Module Go.
     { fs: FS.State;
       maillocks: Globals.State (slice.t LockRef); }.
 
-  Global Instance etaState : Settable _ := settable! Build_State <fs; maillocks>.
+  Global Instance etaState : Settable _ := settable! Build_State <fs; maillocks >.
 
   Definition step T (op:Op T) : relation State State T :=
     match op with
     | FilesysOp op => _zoom fs (FS.step op)
     | DataOp op => _zoom fs (_zoom FS.heap (Data.step op))
     | LockGlobalOp op => _zoom maillocks (Globals.step op)
+    | DiskOp op => error
     end.
 
   Import RelationNotations.
