src/Goose/Disk.v
@@ -1,0 +1,75 @@
+From RecordUpdate Require Import RecordSet.
+From Tactical Require Import ProofAutomation.
+
+From Perennial Require Import Spec.Proc.
+From Perennial Require Import Spec.InjectOp.
+From Perennial Require Import Spec.SemanticsHelpers.
+From Perennial Require Import Spec.LockDefs.
+From Perennial.Goose Require Import Machine.
+From Perennial.Goose Require Import GoZeroValues.
+From Perennial.Goose Require Import Heap.
+
+From Classes Require Import EqualDec.
+From stdpp Require Import fin_maps.
+
+From Transitions Require Import Relations.
+
+Import EqualDecNotation.
+
+Definition BlockSize : uint64 := 4096.
+Opaque BlockSize.
+Definition Block {model:GoModel} := slice.t byte.
+
+Module Disk.
+  Section GoModel.
+  Context `{model_wf:GoModelWf}.
+
+  Implicit Types (a:uint64) (v:Block).
+
+  (* the types of the arguments are determined by their name, using the implicit
+  types given above *)
+  Inductive Op : Type -> Type :=
+  | Read a : Op Block
+  | Write a v : Op unit
+  | Size : Op uint64
+  | Barrier : Op unit
+  .
+
+  Section OpWrappers.
+
+    Context {Op'} {i:Injectable Op Op'}.
+    Notation proc := (proc Op').
+    Notation "'Call!' op" := (Call (inject op) : proc _) (at level 0, op at level 200).
+    Definition read a : proc _ := Call! Read a.
+    Definition write a v : proc _ := Call! Write a v.
+    Definition size : proc _ := Call! Size.
+    Definition barrier : proc _ := Call! Barrier.
+
+  End OpWrappers.
+
+  Record State :=
+    mkState { blocks: list Block; }.
+
+  Global Instance _eta : Settable State :=
+    settable! mkState <blocks>.
+
+  Import RelationNotations.
+
+  Definition step T (op:Op T) : relation State State T :=
+    error.
+
+  Definition crash_step : relation State State unit :=
+    pure tt.
+
+  Theorem crash_step_non_err s res :
+      crash_step s res ->
+      res <> Err.
+  Proof.
+    destruct res; eauto.
+  Qed.
+
+  Global Instance empty_disk : Empty State :=
+    {| blocks := nil; |}.
+
+  End GoModel.
+End Disk.
